AstToCfgCorrectness.dfy
@@ -1,4 +1,5 @@
 include "AstToCfg_simple.dfy"
+include "Util.dfy"
 
 
 module AstToCfgCorrectness
@@ -16,7 +17,7 @@ module AstToCfgCorrectness
     ensures 
       var (cfg, nextVersion', exitOpt) := AstToCfgAux(c, nextVersion); 
       var exit := exitOpt.value; //DISCUSS: does not work if replace {exit} by {exitOpt.value}
-      IsAcyclic(cfg.successors, cfg.entry, CoveringSet2(nextVersion, nextVersion', {exit}))
+      IsAcyclic(cfg.successors, cfg.entry, CoveringSet(nextVersion, nextVersion', {exit}))
   {
     AstToCfgAcyclic(c, nextVersion);
   }
@@ -26,7 +27,7 @@ module AstToCfgCorrectness
     requires IsAcyclic(cfg.successors, n, cover1)
     requires IsAcyclic(cfg.successors, n, cover2)
     ensures WpCfg(a, cfg, n, post, cover1) == WpCfg(a, cfg, n, post, cover2)
-   
+ 
   lemma AstToCfgSemanticsPreservation<A(!new)>(
     a: absval_interp<A>,
     c: Cmd, 
@@ -38,24 +39,27 @@ module AstToCfgCorrectness
     ensures 
       var (cfg, nextVersion', exitOpt):= AstToCfgAux(c, nextVersion); 
       var exit := exitOpt.value;
-      var cover' := CoveringSet2(nextVersion, nextVersion', {exitOpt.value});
+      var cover' := CoveringSet(nextVersion, nextVersion', {exitOpt.value});
 
-      IsAcyclic(cfg.successors, cfg.entry, CoveringSet2(nextVersion, nextVersion', {exitOpt.value})) ==> 
+      IsAcyclic(cfg.successors, cfg.entry, CoveringSet(nextVersion, nextVersion', {exitOpt.value})) ==> 
         WpShallow(a, c, post)(s) == WpCfg(a, cfg, cfg.entry, post.normal, cover')(s);
     {
       match c {
         case SimpleCmd(sc) => 
         case Seq(c1, c2) =>
+          assume false; //TODO: remove (just used to speed up verification of if-proof development)
           var (cfg1, nextVersion1, exitOpt1) := AstToCfgAux(c1, nextVersion);
           var exit1 := exitOpt1.value;
           
           var (cfg2, nextVersion2, exitOpt2) := AstToCfgAux(c2, nextVersion1);
           var exit2 := exitOpt2.value; 
 
-          var cover1 := CoveringSet2(nextVersion, nextVersion1, {exitOpt1.value});
-          var cover2 := CoveringSet2(nextVersion1, nextVersion2, {exitOpt2.value});
-          var cover3 := CoveringSet2(nextVersion, nextVersion2, {exitOpt2.value});
-          assert cover1 + cover2 <= cover3;
+          var cover1 := CoveringSet(nextVersion, nextVersion1, {exitOpt1.value});
+          var cover2 := CoveringSet(nextVersion1, nextVersion2, {exitOpt2.value});
+          var cover3 := CoveringSet(nextVersion, nextVersion2, {exitOpt2.value});
+          assert cover1 + cover2 <= cover3 by {
+            reveal CoveringSet();
+          }
 
           var successors := (cfg1.successors + cfg2.successors)[exitOpt1.value := [cfg2.entry]];
 
@@ -85,22 +89,132 @@ module AstToCfgCorrectness
               }
               WpCfg(a, cfg1, cfg1.entry, WpCfg(a, cfg2, cfg2.entry, post.normal, cover2), cover1)(s); 
                 { 
+                  reveal CoveringSet();
 
                   assert cfg1.blocks.Keys == cfg1.successors.Keys + {exitOpt1.value};
                   assert cfg2.blocks.Keys == cfg2.successors.Keys + {exitOpt2.value};
-                  assert cfg1.successors.Keys <= CoveringSet2(nextVersion, nextVersion1, {exit1});
-                  assert cfg2.successors.Keys <= CoveringSet2(nextVersion1, nextVersion2, {exit1});
-                  assert CoveringSet2(nextVersion, nextVersion1, {}) !! CoveringSet2(nextVersion1, nextVersion2, {});
+                  assert cfg1.successors.Keys <= CoveringSet(nextVersion, nextVersion1, {exit1}); 
+                  assert cfg2.successors.Keys <= CoveringSet(nextVersion1, nextVersion2, {exit1}); 
+                  assert CoveringSet(nextVersion, nextVersion1, {}) !! CoveringSet(nextVersion1, nextVersion2, {}); 
                   assert cover3 == cover1+cover2+{exit1};
                   
+                  assert cfg1.blocks.Keys !! cover2;
+
                   WpCfgMerge(a, cfg1, cfg2, cfg1.entry, exit1, post.normal, cover1, cover2);
                 }
               WpCfg(a, cfg', cfg1.entry, post.normal, cover3)(s);
             }
           }         
-        case _ => assume false;
-      }
+        case If(optCond, thn, els) =>
+          //assume false;
+          assume optCond == None; //TODO: simple case first, then handle other case
 
+          /** CFG thn branch */
+          var (entry, entryBlock) := (nextVersion, Skip);
+          var (cfgThn, nextVersion1, exitOpt1) := AstToCfgAux(thn, entry+1);
+
+          var cfgThn' := 
+            if optCond.Some? then
+              Cfg(cfgThn.entry, cfgThn.blocks[cfgThn.entry := SeqSimple(Assume(optCond.value), cfgThn.blocks[cfgThn.entry])], cfgThn.successors)
+            else
+              cfgThn;
+
+          /** CFG els branch */
+          var (cfgEls, nextVersion2, exitOpt2) := AstToCfgAux(els, nextVersion1);
+
+          var cfgEls' := 
+            if optCond.Some? then
+              Cfg(cfgEls.entry, cfgEls.blocks[cfgEls.entry := SeqSimple(Assume(UnOp(Not, optCond.value)), cfgEls.blocks[cfgEls.entry])], cfgEls.successors)
+            else
+              cfgEls;
+
+          var (thnEntry, thnS) := (cfgThn.entry, cfgThn.successors);
+          var thnExit := exitOpt1.value;
+
+          var cover1 := CoveringSet(nextVersion+1, nextVersion1, {thnExit});
+          AstToCfgAcyclic(thn, entry+1);
+          assert IsAcyclic(thnS, thnEntry, cover1);
+
+          var (elsEntry, elsS) := (cfgEls.entry, cfgEls.successors);
+          var elsExit := exitOpt2.value;
+
+          var cover2 := CoveringSet(nextVersion1, nextVersion2, {elsExit});
+          AstToCfgAcyclic(els, nextVersion1);
+          assert IsAcyclic(elsS, elsEntry, cover2);
+
+          var blocksBeforeJoin := (cfgThn'.blocks + cfgEls'.blocks)[entry := Skip];
+          var successorsBeforeJoin := (cfgThn'.successors + cfgEls'.successors)[entry := [cfgThn'.entry, cfgEls'.entry]];
+
+          var (joinId, joinBlock) := (nextVersion2, Skip);
+
+          /** result data */
+          var blocks := blocksBeforeJoin[joinId := joinBlock];
+          var successors := successorsBeforeJoin[thnExit := [joinId]][elsExit := [joinId]];
+          var cfg' := Cfg(entry, blocks, successors);
+          var cover3 := CoveringSet(nextVersion, nextVersion2+1, {joinId});
+
+          /** lift thn branch WP to entire CFG */
+          calc {
+            WpShallow(a, thn, post)(s);
+            WpCfg(a, cfgThn', cfgThn'.entry, post.normal, cover1)(s);
+              { WpCfgEntryIndep(a, cfgThn', entry, cfgThn'.entry, post.normal, cover1); }
+            WpCfg(a, Cfg(entry, cfgThn'.blocks, cfgThn'.successors), cfgThn'.entry, post.normal, cover1)(s);
+              {assume false;}
+            WpCfg(a, Cfg(entry, cfgThn'.blocks + cfgEls'.blocks, cfgThn'.successors + cfgEls'.successors), cfgThn'.entry, post.normal, cover1)(s);
+              {assume false;}
+            WpCfg(a, Cfg(entry, blocksBeforeJoin, successorsBeforeJoin), cfgThn'.entry, post.normal, cover1)(s);
+              {assume false;}
+            WpCfg(a, Cfg(entry, blocks, successorsBeforeJoin[thnExit := [joinId]]), cfgThn'.entry, post.normal, cover1)(s);
+              {assume false;}
+            WpCfg(a, cfg', cfgThn'.entry, post.normal, cover1)(s);
+              {assume false;}
+            WpCfg(a, cfg', cfgThn'.entry, post.normal, cover3-{entry})(s);
+          }
+
+          assume false;
+
+          /** lift els branch WP to entire CFG */
+          calc {
+            WpShallow(a, els, post)(s);
+              {assume false;}
+            WpCfg(a, cfg', cfgEls'.entry, post.normal, cover2)(s);
+              {assume false;}
+            WpCfg(a, cfg', cfgEls'.entry, post.normal, cover3-{entry})(s);
+          }
+
+
+          /*
+          var (cfg, nextVersion', exitOpt) := AstToCfgAux(c, nextVersion); 
+
+          assume cfg'.successors == cfg.successors; //TODO: switch to assert
+          assume cfg == cfg'; //TODO: switch to assert
+          */
+
+          var (cfg, nextVersion', exitOpt):= AstToCfgAux(c, nextVersion); 
+          var exit := exitOpt.value;
+          var cover' := CoveringSet(nextVersion, nextVersion', {exitOpt.value});
+
+          /*IsAcyclic(cfg.successors, cfg.entry, CoveringSet(nextVersion, nextVersion', {exitOpt.value})) ==> 
+            WpShallow(a, c, post)(s) == WpCfg(a, cfg, cfg.entry, post.normal, cover')(s);*/
+          
+          assert nextVersion' == nextVersion2+1;
+          assert cfg'.successors == cfg.successors; //TODO: switch to assert
+          assert cfg == cfg'; //TODO: switch to assert
+
+          if IsAcyclic(cfg'.successors, cfg'.entry, cover3) {
+            calc {
+              WpCfg(a, cfg', cfg'.entry, post.normal, cover3)(s);
+                { assert cfg'.blocks[entry] == Skip;
+                  assert cfg'.successors[entry] ==  [cfgThn'.entry, cfgEls'.entry];
+                }
+              WpShallowSimpleCmd(a, Skip, WpCfgConjunction(a, cfg', [cfgThn'.entry, cfgEls'.entry], post.normal, cover3-{entry}))(s);
+              WpCfgConjunction(a, cfg', [cfgThn'.entry, cfgEls'.entry], post.normal, cover3-{entry})(s);
+              Util.AndOpt(WpCfg(a, cfg', cfgThn'.entry, post.normal, cover3-{entry})(s), WpCfg(a, cfg', cfgEls'.entry, post.normal, cover3-{entry})(s));
+              Util.AndOpt(WpShallow(a, thn, post)(s), WpShallow(a, els, post)(s));
+              WpShallow(a, c, post)(s);
+            }
+          }
+      }
     }
 
 }
